Defined Semantics & Proof skeleton

cfrontend/Cexec.v
@@ -673,7 +673,7 @@ Qed.
 Inductive reduction: Type :=
   | Lred (rule: string) (l': expr) (m': mem)
   | Rred (rule: string) (r': expr) (m': mem) (t: trace)
-  | Callred (rule: string) (fd: fundef) (args: list val) (tyres: type) (m': mem)
+  | Callred (rule: string) (fd: fundef) (args: list val) (tyres: type) (m': mem) (id:ident)
   | Stuckred.
 
 Section EXPRS.
@@ -729,6 +729,12 @@ Notation " 'check' A ; B" := (if A then B else stuck)
   : reducts_monad_scope.
 
 Local Open Scope reducts_monad_scope.
+
+Definition invert_pointer vf :=
+  match vf with
+  | Vptr (Global id) ofs => if Ptrofs.eq ofs Ptrofs.zero then Some id else None
+  | _ => None
+  end.
 
 Fixpoint step_expr (k: kind) (a: expr) (m: mem): reducts expr :=
   match k, a with
@@ -902,10 +908,11 @@ Fixpoint step_expr (k: kind) (a: expr) (m: mem): reducts expr :=
       | Some(vf, tyf), Some vtl =>
           match classify_fun tyf with
           | fun_case_f tyargs tyres cconv =>
+              do id <- invert_pointer vf;
               do fd <- Genv.find_funct ge vf;
               do vargs <- sem_cast_arguments vtl tyargs m;
               check type_eq (type_of_fundef fd) (Tfunction tyargs tyres cconv);
-              topred (Callred "red_call" fd vargs ty m)
+              topred (Callred "red_call" fd vargs ty m id)
           | _ => stuck
           end
       | _, _ =>
@@ -950,8 +957,8 @@ Inductive imm_safe_t: kind -> expr -> mem -> Prop :=
       rred ge r m t r' m' -> possible_trace w t w' ->
       context RV to C ->
       imm_safe_t to (C r) m
-  | imm_safe_t_callred: forall to C r m fd args ty,
-      callred ge r m fd args ty ->
+  | imm_safe_t_callred: forall to C r m fd args ty id,
+      callred ge r m fd args ty id->
       context RV to C ->
       imm_safe_t to (C r) m.
 
@@ -1019,8 +1026,9 @@ Definition invert_expr_prop (a: expr) (m: mem) : Prop :=
       exists v, sem_cast v1 ty1 tycast m = Some v
   | Ecall (Eval vf tyf) rargs ty =>
       exprlist_all_values rargs ->
-      exists tyargs tyres cconv fd vl,
-         classify_fun tyf = fun_case_f tyargs tyres cconv
+      exists tyargs tyres cconv fd vl id,
+         vf = Vptr (Global id) Ptrofs.zero
+      /\ classify_fun tyf = fun_case_f tyargs tyres cconv
       /\ Genv.find_funct ge vf = Some fd
       /\ cast_arguments m rargs tyargs vl
       /\ type_of_fundef fd = Tfunction tyargs tyres cconv
@@ -1063,12 +1071,12 @@ Proof.
 Qed.
 
 Lemma callred_invert:
-  forall r fd args ty m,
-  callred ge r m fd args ty ->
+  forall r fd args ty m id,
+  callred ge r m fd args ty id ->
   invert_expr_prop r m.
 Proof.
   intros. inv H. simpl.
-  intros. exists tyargs, tyres, cconv, fd, args; auto.
+  intros. exists tyargs, tyres, cconv, fd, args, id; auto.
 Qed.
 
 Scheme context_ind2 := Minimality for context Sort Prop
@@ -1160,7 +1168,7 @@ Definition reduction_ok (k: kind) (a: expr) (m: mem) (rd: reduction) : Prop :=
   match k, rd with
   | LV, Lred _ l' m' => lred ge e a m l' m'
   | RV, Rred _ r' m' t => rred ge a m t r' m' /\ exists w', possible_trace w t w'
-  | RV, Callred _ fd args tyres m' => callred ge a m fd args tyres /\ m' = m
+  | RV, Callred _ fd args tyres m' id => callred ge a m fd args tyres id /\ m' = m
   | LV, Stuckred => ~imm_safe_t k a m
   | RV, Stuckred => ~imm_safe_t k a m
   | _, _ => False
@@ -1513,15 +1521,21 @@ Proof with (try (apply not_invert_ok; simpl; intro; myinv; intuition congruence;
   rewrite (is_val_inv _ _ _ Heqo). exploit is_val_list_all_values; eauto. intros ALLVAL.
   (* top *)
   destruct (classify_fun tyf) as [tyargs tyres cconv|] eqn:?...
+  destruct (invert_pointer vf) as [id|] eqn:?...
   destruct (Genv.find_funct ge vf) as [fd|] eqn:?...
   destruct (sem_cast_arguments vtl tyargs m) as [vargs|] eqn:?...
   destruct (type_eq (type_of_fundef fd) (Tfunction tyargs tyres cconv))...
   apply topred_ok; auto. red. split; auto. eapply red_call; eauto.
+  unfold invert_pointer in Heqo1. repeat destr_in Heqo1.
+  apply Ptrofs.same_if_eq in Heqb1. congruence.
   eapply sem_cast_arguments_sound; eauto.
   apply not_invert_ok; simpl; intros; myinv. specialize (H ALLVAL). myinv. congruence.
   apply not_invert_ok; simpl; intros; myinv. specialize (H ALLVAL). myinv.
   exploit sem_cast_arguments_complete; eauto. intros [vtl' [P Q]]. congruence.
   apply not_invert_ok; simpl; intros; myinv. specialize (H ALLVAL). myinv. congruence.
+  apply not_invert_ok; simpl; intros; myinv. specialize (H ALLVAL). myinv.
+  destruct vf eqn: Hvf; simpl in *; try congruence. repeat destr_in Heqo1.
+  generalize (Ptrofs.eq_spec i Ptrofs.zero). rewrite Heqb1. intro. congruence.
   apply not_invert_ok; simpl; intros; myinv. specialize (H ALLVAL). myinv. congruence.
   (* depth *)
   eapply incontext2_list_ok; eauto.
@@ -1642,13 +1656,14 @@ Proof.
 Qed.
 
 Lemma callred_topred:
-  forall a fd args ty m,
-  callred ge a m fd args ty ->
-  exists rule, step_expr RV a m = topred (Callred rule fd args ty m).
+  forall a fd args ty m id,
+  callred ge a m fd args ty id->
+  exists rule, step_expr RV a m = topred (Callred rule fd args ty m id).
 Proof.
   induction 1; simpl.
-  rewrite H2. exploit sem_cast_arguments_complete; eauto. intros [vtl [A B]].
-  rewrite A; rewrite H; rewrite B; rewrite H1; rewrite dec_eq_true. econstructor; eauto.
+  rewrite H3. exploit sem_cast_arguments_complete; eauto. intros [vtl [A B]].
+  assert (invert_pointer vf = Some id). rewrite H. auto.
+  rewrite A; rewrite H4; rewrite H0; rewrite B; rewrite H2; rewrite dec_eq_true. econstructor; eauto.
 Qed.
 
 Definition reducts_incl {A B: Type} (C: A -> B) (res1: reducts A) (res2: reducts B) : Prop :=
@@ -1962,7 +1977,7 @@ Definition expr_final_state (f: function) (k: cont) (e: env) (C_rd: (expr -> exp
   match snd C_rd with
   | Lred rule a m => TR rule E0 (ExprState f (fst C_rd a) k e m)
   | Rred rule a m t => TR rule t (ExprState f (fst C_rd a) k e m)
-  | Callred rule fd vargs ty m => TR rule E0 (Callstate fd vargs (Kcall f e (fst C_rd) ty k) m)
+  | Callred rule fd vargs ty m id => TR rule E0 (Callstate fd vargs (Kcall f e (fst C_rd) ty k) m id)
   | Stuckred => TR "step_stuck" E0 Stuckstate
   end.
 
@@ -2000,7 +2015,8 @@ Definition do_step (w: world) (s: state) : list transition :=
         | Kreturn k =>
             do v' <- sem_cast v ty f.(fn_return) m;
             do m' <- Mem.free_list m (blocks_of_env ge e);
-            ret "step_return_2" (Returnstate v' (call_cont k) m')
+            do m'' <- Mem.return_frame m';
+            ret "step_return_2" (Returnstate v' (call_cont k) m'')
         | Kswitch1 sl k =>
             do n <- sem_switch_arg v ty;
             ret "step_expr_switch" (State f (seq_of_labeled_statement (select_switch n sl)) (Kswitch2 k) e m)
@@ -2052,12 +2068,14 @@ Definition do_step (w: world) (s: state) : list transition :=
 
   | State f (Sreturn None) k e m =>
       do m' <- Mem.free_list m (blocks_of_env ge e);
-      ret "step_return_0" (Returnstate Vundef (call_cont k) m')
+      do m'' <- Mem.return_frame m';
+      ret "step_return_0" (Returnstate Vundef (call_cont k) m'')
   | State f (Sreturn (Some x)) k e m =>
       ret "step_return_1" (ExprState f x (Kreturn k) e m)
   | State f Sskip ((Kstop | Kcall _ _ _ _ _) as k) e m =>
       do m' <- Mem.free_list m (blocks_of_env ge e);
-      ret "step_skip_call" (Returnstate Vundef k m')
+      do m'' <- Mem.return_frame m';
+      ret "step_skip_call" (Returnstate Vundef k m'')
 
   | State f (Sswitch x sl) k e m =>
       ret "step_switch" (ExprState f x (Kswitch1 sl k) e m)
@@ -2074,12 +2092,13 @@ Definition do_step (w: world) (s: state) : list transition :=
       | None => nil
       end
 
-  | Callstate (Internal f) vargs k m =>
+  | Callstate (Internal f) vargs k m id =>
       check (list_norepet_dec ident_eq (var_names (fn_params f) ++ var_names (fn_vars f)));
-      let (e,m1) := do_alloc_variables empty_env m (f.(fn_params) ++ f.(fn_vars)) in
+      let (m0,path) := Mem.alloc_frame m id in
+      let (e,m1) := do_alloc_variables empty_env m0 (f.(fn_params) ++ f.(fn_vars)) in
       do m2 <- sem_bind_parameters w e m1 f.(fn_params) vargs;
       ret "step_internal_function" (State f f.(fn_body) k e m2)
-  | Callstate (External ef _ _ _) vargs k m =>
+  | Callstate (External ef _ _ _) vargs k m id =>
       match do_external ef w vargs m with
       | None => nil
       | Some(w',t,v,m') => TR "step_external_function" t (Returnstate v k m') :: nil
@@ -2108,7 +2127,7 @@ Ltac myinv :=
   end.
 
 Local Hint Extern 3 => exact I : core.
-
+Local Opaque Mem.alloc_frame.
 Theorem do_step_sound:
   forall w S rule t S',
   In (TR rule t S') (do_step w S) ->
@@ -2149,9 +2168,11 @@ Proof with try (left; right; econstructor; eauto; fail).
 (* callstate *)
   destruct fd; myinv.
   (* internal *)
-  destruct (do_alloc_variables empty_env m (fn_params f ++ fn_vars f)) as [e m1] eqn:?.
-  myinv. left; right; apply step_internal_function with m1. auto.
-  change e with (fst (e,m1)). change m1 with (snd (e,m1)) at 2. rewrite <- Heqp.
+  destruct (Mem.alloc_frame m id) as [m0 path] eqn:?.
+  destruct (do_alloc_variables empty_env m0 (fn_params f ++ fn_vars f)) as [e m1] eqn:?.
+  myinv. left; right; eapply step_internal_function. eauto. eauto.
+  instantiate (1:= m1).
+  change e with (fst (e,m1)). change m1 with (snd (e,m1)) at 2. rewrite <- Heqp0.
   apply do_alloc_variables_sound. eapply sem_bind_parameters_sound; eauto.
   (* external *)
   destruct p as [[[w' tr] v] m']. myinv. left; right; constructor.
@@ -2206,7 +2227,7 @@ Proof with (unfold ret; eauto with coqlib).
   unfold do_step; rewrite NOTVAL.
   exploit callred_topred; eauto. instantiate (1 := w). instantiate (1 := e).
   intros (rule & STEP). exists rule.
-  change (TR rule E0 (Callstate fd vargs (Kcall f e C ty k) m)) with (expr_final_state f k e (C, Callred rule fd vargs ty m)).
+  change (TR rule E0 (Callstate fd vargs (Kcall f e C ty k) m id)) with (expr_final_state f k e (C, Callred rule fd vargs ty m id)).
   apply in_map.
   generalize (step_expr_context e w _ _ _ H1 a m). unfold reducts_incl.
   intro. replace C with (fun x => C x). apply H2.
@@ -2233,16 +2254,18 @@ Proof with (unfold ret; eauto with coqlib).
   rewrite H0...
   rewrite H0...
   destruct H0; subst x...
-  rewrite H0...
   rewrite H0; rewrite H1...
-  rewrite H1. red in H0. destruct k; try contradiction...
+  rewrite H0; rewrite H1; rewrite H2...
+  rewrite H1. rewrite H2. red in H0. destruct k; try contradiction...
   rewrite H0...
   destruct H0; subst x...
   rewrite H0...
 
   (* Call step *)
-  rewrite pred_dec_true; auto. rewrite (do_alloc_variables_complete _ _ _ _ _ H1).
-  rewrite (sem_bind_parameters_complete _ _ _ _ _ _ H2)...
+  rewrite pred_dec_true; auto.
+  rewrite H1.
+  rewrite (do_alloc_variables_complete _ _ _ _ _ H2).
+  rewrite (sem_bind_parameters_complete _ _ _ _ _ _ H3)...
   exploit do_ef_external_complete; eauto. intro EQ; rewrite EQ. auto with coqlib.
 Qed.
 
@@ -2256,7 +2279,7 @@ Definition do_initial_state (p: program): option (genv * state) :=
   do b <- Genv.find_symbol ge p.(prog_main);
   do f <- Genv.find_funct_ptr ge b;
   check (type_eq (type_of_fundef f) (Tfunction Tnil type_int32s cc_default));
-  Some (ge, Callstate f nil Kstop m0).
+  Some (ge, Callstate f nil Kstop m0 p.(prog_main)).
 
 Definition at_final_state (S: state): option int :=
   match S with
