cfrontend/Csharpminor.v
@@ -159,7 +159,8 @@ Inductive state: Type :=
       forall (f: fundef)                (**r function to invoke *)
              (args: list val)           (**r arguments provided by caller *)
              (k: cont)                  (**r what to do next  *)
-             (m: mem),                  (**r memory state *)
+             (m: mem)                   (**r memory state *)
+             (id: ident),
       state
   | Returnstate:                (**r Return from a function *)
       forall (v: val)                   (**r Return value *)
@@ -364,11 +365,12 @@ Inductive step: state -> trace -> state -> Prop :=
   | step_skip_block: forall f k e le m,
       step (State f Sskip (Kblock k) e le m)
         E0 (State f Sskip k e le m)
-  | step_skip_call: forall f k e le m m',
+  | step_skip_call: forall f k e le m m' m'',
       is_call_cont k ->
       Mem.free_list m (blocks_of_env e) = Some m' ->
+      Mem.return_frame m' = Some m'' ->
       step (State f Sskip k e le m)
-        E0 (Returnstate Vundef k m')
+        E0 (Returnstate Vundef k m'')
 
   | step_set: forall f id a k e le m v,
       eval_expr e le m a v ->
@@ -382,13 +384,14 @@ Inductive step: state -> trace -> state -> Prop :=
       step (State f (Sstore chunk addr a) k e le m)
         E0 (State f Sskip k e le m')
 
-  | step_call: forall f optid sig a bl k e le m vf vargs fd,
+  | step_call: forall f optid sig a bl k e le m vf vargs fd id,
+      vf = Vptr (Global id) Ptrofs.zero ->
       eval_expr e le m a vf ->
       eval_exprlist e le m bl vargs ->
       Genv.find_funct ge vf = Some fd ->
       funsig fd = sig ->
       step (State f (Scall optid sig a bl) k e le m)
-        E0 (Callstate fd vargs (Kcall optid f e le k) m)
+        E0 (Callstate fd vargs (Kcall optid f e le k) m id)
 
   | step_builtin: forall f optid ef bl k e le m vargs t vres m',
       eval_exprlist e le m bl vargs ->
@@ -430,15 +433,17 @@ Inductive step: state -> trace -> state -> Prop :=
       step (State f (Sswitch islong a cases) k e le m)
         E0 (State f (seq_of_lbl_stmt (select_switch n cases)) k e le m)
 
-  | step_return_0: forall f k e le m m',
+  | step_return_0: forall f k e le m m' m'',
       Mem.free_list m (blocks_of_env e) = Some m' ->
+      Mem.return_frame m' = Some m'' ->
       step (State f (Sreturn None) k e le m)
-        E0 (Returnstate Vundef (call_cont k) m')
-  | step_return_1: forall f a k e le m v m',
+        E0 (Returnstate Vundef (call_cont k) m'')
+  | step_return_1: forall f a k e le m v m' m'',
       eval_expr e le m a v ->
       Mem.free_list m (blocks_of_env e) = Some m' ->
+      Mem.return_frame m' = Some m'' ->
       step (State f (Sreturn (Some a)) k e le m)
-        E0 (Returnstate v (call_cont k) m')
+        E0 (Returnstate v (call_cont k) m'')
   | step_label: forall f lbl s k e le m,
       step (State f (Slabel lbl s) k e le m)
         E0 (State f s k e le m)
@@ -448,18 +453,19 @@ Inductive step: state -> trace -> state -> Prop :=
       step (State f (Sgoto lbl) k e le m)
         E0 (State f s' k' e le m)
 
-  | step_internal_function: forall f vargs k m m1 e le,
+  | step_internal_function: forall f vargs k m m0 m1 e le id path,
       list_norepet (map fst f.(fn_vars)) ->
       list_norepet f.(fn_params) ->
       list_disjoint f.(fn_params) f.(fn_temps) ->
-      alloc_variables empty_env m (fn_vars f) e m1 ->
+      Mem.alloc_frame m id = (m0,path) ->
+      alloc_variables empty_env m0 (fn_vars f) e m1 ->
       bind_parameters f.(fn_params) vargs (create_undef_temps f.(fn_temps)) = Some le ->
-      step (Callstate (Internal f) vargs k m)
+      step (Callstate (Internal f) vargs k m id)
         E0 (State f f.(fn_body) k e le m1)
 
-  | step_external_function: forall ef vargs k m t vres m',
+  | step_external_function: forall ef vargs k m t vres m' id,
       external_call ef ge vargs m t vres m' ->
-      step (Callstate (External ef) vargs k m)
+      step (Callstate (External ef) vargs k m id)
          t (Returnstate vres k m')
 
   | step_return: forall v optid f e le k m,
@@ -480,7 +486,7 @@ Inductive initial_state (p: program): state -> Prop :=
       Genv.find_symbol ge p.(prog_main) = Some b ->
       Genv.find_funct_ptr ge b = Some f ->
       funsig f = signature_main ->
-      initial_state p (Callstate f nil Kstop m0).
+      initial_state p (Callstate f nil Kstop m0 p.(prog_main)).
 
 (** A final state is a [Returnstate] with an empty continuation. *)
 
