cfrontend/Cshmgenproof.v
@@ -1403,14 +1403,14 @@ Inductive match_states: Clight.state -> Csharpminor.state -> Prop :=
       match_states (Clight.State f s k e le m)
                    (State tf ts' tk' te le m)
   | match_callstate:
-      forall fd args k m tfd tk targs tres cconv cu ce
+      forall fd args k m tfd tk targs tres cconv cu ce id
           (LINK: linkorder cu prog)
           (TR: match_fundef cu fd tfd)
           (MK: match_cont ce tres 0%nat 0%nat k tk)
           (ISCC: Clight.is_call_cont k)
           (TY: type_of_fundef fd = Tfunction targs tres cconv),
-      match_states (Clight.Callstate fd args k m)
-                   (Callstate tfd args tk m)
+      match_states (Clight.Callstate fd args k m id)
+                   (Callstate tfd args tk m id)
   | match_returnstate:
       forall res tres k m tk ce
           (MK: match_cont ce tres 0%nat 0%nat k tk)
@@ -1591,7 +1591,7 @@ Proof.
                 sig_cc := cc |}) in *.
   assert (SIG: funsig tfd = sg).
   { unfold sg; erewrite typlist_of_arglist_eq by eauto.
-    eapply transl_fundef_sig1; eauto. rewrite H3; auto. }
+    eapply transl_fundef_sig1; eauto. rewrite H4; auto. }
   assert (EITHER: tk' = tk /\ ts' = Scall optid sg x x0
                \/ exists id, optid = Some id /\
                   tk' = tk /\ ts' = Sseq (Scall optid sg x x0)
@@ -1601,7 +1601,7 @@ Proof.
     inv MTR. right; exists i; auto.
     inv MTR; auto.
     inv MTR; auto. }
-  destruct EITHER as [(EK & ES) | (id & EI & EK & ES)]; rewrite EK, ES.
+  destruct EITHER as [(EK & ES) | (id' & EI & EK & ES)]; rewrite EK, ES.
   + (* without normalization of return value *)
     econstructor; split.
     apply plus_one. eapply step_call; eauto.
@@ -1713,7 +1713,7 @@ Proof.
 - (* return none *)
   monadInv TR. inv MTR.
   econstructor; split.
-  apply plus_one. constructor.
+  apply plus_one. econstructor; eauto.
   eapply match_env_free_blocks; eauto.
   eapply match_returnstate with (ce := prog_comp_env cu); eauto.
   eapply match_cont_call_cont. eauto.
@@ -1722,7 +1722,7 @@ Proof.
 - (* return some *)
   monadInv TR. inv MTR.
   econstructor; split.
-  apply plus_one. constructor.
+  apply plus_one. econstructor; eauto.
   eapply make_cast_correct; eauto. eapply transl_expr_correct; eauto.
   eapply match_env_free_blocks; eauto.
   eapply match_returnstate with (ce := prog_comp_env cu); eauto.
@@ -1733,8 +1733,8 @@ Proof.
   monadInv TR. inv MTR.
   exploit match_cont_is_call_cont; eauto. intros [A B].
   econstructor; split.
-  apply plus_one. apply step_skip_call. auto.
-  eapply match_env_free_blocks; eauto.
+  apply plus_one. eapply step_skip_call. eauto.
+  eapply match_env_free_blocks; eauto. eauto.
   eapply match_returnstate with (ce := prog_comp_env cu); eauto.
   constructor.
 
@@ -1785,7 +1785,7 @@ Proof.
   econstructor; eauto. constructor.
 
 - (* internal function *)
-  inv H. inv TR. monadInv H5.
+  inv H. inv TR. monadInv H6.
   exploit match_cont_is_call_cont; eauto. intros [A B].
   exploit match_env_alloc_variables; eauto.
   apply match_env_empty.
@@ -1795,6 +1795,7 @@ Proof.
   simpl. erewrite transl_vars_names by eauto. assumption.
   simpl. assumption.
   simpl. assumption.
+  eauto. eauto.
   simpl; eauto.
   simpl. rewrite create_undef_temps_match. eapply bind_parameter_temps_match; eauto.
   simpl. econstructor; eauto.
@@ -1841,6 +1842,7 @@ Proof.
   { eapply transl_fundef_sig2; eauto. }
   econstructor; split.
   econstructor; eauto. apply (Genv.init_mem_match TRANSL). eauto.
+  destruct TRANSL as (P & Q & R). rewrite Q.
   econstructor; eauto. instantiate (1 := prog_comp_env cu). constructor; auto. exact I.
 Qed.
 
