cfrontend/Cstrategy.v
@@ -362,7 +362,8 @@ Inductive estep: state -> trace -> state -> Prop :=
       estep (ExprState f (C (Eparen r tycast ty)) k e m)
          E0 (ExprState f (C (Eval v ty)) k e m)
 
-  | step_call: forall f C rf rargs ty k e m targs tres cconv vf vargs fd,
+  | step_call: forall f C rf rargs ty k e m targs tres cconv vf vargs fd id,
+      vf = Vptr (Global id) Ptrofs.zero ->
       leftcontext RV RV C ->
       classify_fun (typeof rf) = fun_case_f targs tres cconv ->
       eval_simple_rvalue e m rf vf ->
@@ -370,7 +371,7 @@ Inductive estep: state -> trace -> state -> Prop :=
       Genv.find_funct ge vf = Some fd ->
       type_of_fundef fd = Tfunction targs tres cconv ->
       estep (ExprState f (C (Ecall rf rargs ty)) k e m)
-         E0 (Callstate fd vargs (Kcall f e C ty k) m)
+         E0 (Callstate fd vargs (Kcall f e C ty k) m id)
 
   | step_builtin: forall f C ef tyargs rargs ty k e m vargs t vres m',
       leftcontext RV RV C ->
@@ -471,7 +472,7 @@ Proof.
 Qed.
 
 Lemma callred_kind:
-  forall a m fd args ty, callred ge a m fd args ty -> expr_kind a = RV.
+  forall a m fd args ty id, callred ge a m fd args ty id-> expr_kind a = RV.
 Proof.
   induction 1; auto.
 Qed.
@@ -563,8 +564,9 @@ Definition invert_expr_prop (a: expr) (m: mem) : Prop :=
       exists v, sem_cast v1 ty1 ty2 m = Some v
   | Ecall (Eval vf tyf) rargs ty =>
       exprlist_all_values rargs ->
-      exists tyargs tyres cconv fd vl,
-         classify_fun tyf = fun_case_f tyargs tyres cconv
+      exists tyargs tyres cconv fd vl id,
+         vf = Vptr (Global id) Ptrofs.zero
+      /\ classify_fun tyf = fun_case_f tyargs tyres cconv
       /\ Genv.find_funct ge vf = Some fd
       /\ cast_arguments m rargs tyargs vl
       /\ type_of_fundef fd = Tfunction tyargs tyres cconv
@@ -606,12 +608,12 @@ Proof.
 Qed.
 
 Lemma callred_invert:
-  forall r fd args ty m,
-  callred ge r m fd args ty ->
+  forall r fd args ty m id,
+  callred ge r m fd args ty id->
   invert_expr_prop r m.
 Proof.
   intros. inv H. simpl.
-  intros. exists tyargs, tyres, cconv, fd, args; auto.
+  intros. exists tyargs, tyres, cconv, fd, args,id; auto.
 Qed.
 
 Scheme context_ind2 := Minimality for context Sort Prop
@@ -1262,7 +1264,7 @@ Proof.
   eapply star_plus_trans.
   eapply eval_simple_rvalue_steps with (C := fun x => C(Ecall x rargs ty)); eauto.
   eapply plus_right.
-  eapply eval_simple_list_steps with (C := fun x => C(Ecall (Eval vf (typeof rf)) x ty)); eauto.
+  eapply eval_simple_list_steps with (C := fun x => C(Ecall (Eval (Vptr (Global id) Ptrofs.zero) (typeof rf)) x ty)); eauto.
   eapply contextlist'_call with (rl0 := Enil); auto.
   left; apply Csem.step_call; eauto. econstructor; eauto.
   traceEq. auto.
@@ -1370,8 +1372,9 @@ Proof.
   eapply safe_steps. eexact S1.
   apply (eval_simple_list_steps f k e m rargs vl E2 C'); auto.
   simpl. intros X. exploit X. eapply rval_list_all_values.
-  intros [tyargs [tyres [cconv [fd [vargs [P [Q [U V]]]]]]]].
-  econstructor; econstructor; eapply step_call; eauto. eapply can_eval_simple_list; eauto.
+  intros [tyargs [tyres [cconv [fd [vargs [id [O[P [Q [U V]]]]]]]]]].
+  econstructor; econstructor; eapply step_call; eauto.
+  eapply can_eval_simple_list; eauto.
 (* builtin *)
   pose (C' := fun x => C(Ebuiltin ef tyargs x ty)).
   assert (contextlist' C'). unfold C'; eapply contextlist'_builtin with (rl0 := Enil); auto.
@@ -1757,14 +1760,15 @@ with eval_expr: env -> mem -> kind -> expr -> trace -> mem -> expr -> Prop :=
       ty = typeof r2 ->
       eval_expr e m RV (Ecomma r1 r2 ty) (t1**t2) m2 r2'
   | eval_call: forall e m rf rargs ty t1 m1 rf' t2 m2 rargs' vf vargs
-                      targs tres cconv fd t3 m3 vres,
+                      targs tres cconv fd t3 m3 vres id,
+      vf = Vptr (Global id) Ptrofs.zero ->
       eval_expr e m RV rf t1 m1 rf' -> eval_exprlist e m1 rargs t2 m2 rargs' ->
       eval_simple_rvalue ge e m2 rf' vf ->
       eval_simple_list ge e m2 rargs' targs vargs ->
       classify_fun (typeof rf) = fun_case_f targs tres cconv ->
       Genv.find_funct ge vf = Some fd ->
       type_of_fundef fd = Tfunction targs tres cconv ->
-      eval_funcall m2 fd vargs t3 m3 vres ->
+      eval_funcall m2 fd vargs t3 m3 vres id->
       eval_expr e m RV (Ecall rf rargs ty) (t1**t2**t3) m3 (Eval vres ty)
 
 with eval_exprlist: env -> mem -> exprlist -> trace -> mem -> exprlist -> Prop :=
@@ -1894,18 +1898,20 @@ with exec_stmt: env -> mem -> statement -> trace -> mem -> outcome -> Prop :=
   function [fd] with arguments [args].  [res] is the value returned
   by the call.  *)
 
-with eval_funcall: mem -> fundef -> list val -> trace -> mem -> val -> Prop :=
-  | eval_funcall_internal: forall m f vargs t e m1 m2 m3 out vres m4,
+with eval_funcall: mem -> fundef -> list val -> trace -> mem -> val -> ident -> Prop :=
+  | eval_funcall_internal: forall m f vargs t e m0 m1 m2 m3 out vres m4 m5 id path,
       list_norepet (var_names f.(fn_params) ++ var_names f.(fn_vars)) ->
-      alloc_variables ge empty_env m (f.(fn_params) ++ f.(fn_vars)) e m1 ->
+      Mem.alloc_frame m id = (m0,path) ->
+      alloc_variables ge empty_env m0 (f.(fn_params) ++ f.(fn_vars)) e m1 ->
       bind_parameters ge e m1 f.(fn_params) vargs m2 ->
       exec_stmt e m2 f.(fn_body) t m3 out ->
       outcome_result_value out f.(fn_return) vres m3 ->
       Mem.free_list m3 (blocks_of_env ge e) = Some m4 ->
-      eval_funcall m (Internal f) vargs t m4 vres
+      Mem.return_frame m4 = Some m5 ->
+      eval_funcall m (Internal f) vargs t m5 vres id
   | eval_funcall_external: forall m ef targs tres cconv vargs t vres m',
       external_call ef ge vargs m t vres m' ->
-      eval_funcall m (External ef targs tres cconv) vargs t m' vres.
+      eval_funcall m (External ef targs tres cconv) vargs t m' vres 1%positive.
 
 Scheme eval_expression_ind5 := Minimality for eval_expression Sort Prop
   with eval_expr_ind5 := Minimality for eval_expr Sort Prop
@@ -2001,14 +2007,15 @@ CoInductive evalinf_expr: env -> mem -> kind -> expr -> traceinf -> Prop :=
       evalinf_exprlist e m1 a2 t2 ->
       evalinf_expr e m RV (Ecall a1 a2 ty) (t1 *** t2)
   | evalinf_call: forall e m rf rargs ty t1 m1 rf' t2 m2 rargs' vf vargs
-                      targs tres cconv fd t3,
+                      targs tres cconv fd t3 id,
+      vf = Vptr (Global id) Ptrofs.zero ->
       eval_expr e m RV rf t1 m1 rf' -> eval_exprlist e m1 rargs t2 m2 rargs' ->
       eval_simple_rvalue ge e m2 rf' vf ->
       eval_simple_list ge e m2 rargs' targs vargs ->
       classify_fun (typeof rf) = fun_case_f targs tres cconv ->
       Genv.find_funct ge vf = Some fd ->
       type_of_fundef fd = Tfunction targs tres cconv ->
-      evalinf_funcall m2 fd vargs t3 ->
+      evalinf_funcall m2 fd vargs t3 id ->
       evalinf_expr e m RV (Ecall rf rargs ty) (t1***t2***t3)
 
 with evalinf_exprlist: env -> mem -> exprlist -> traceinf -> Prop :=
@@ -2116,13 +2123,14 @@ with execinf_stmt: env -> mem -> statement -> traceinf -> Prop :=
 (** [evalinf_funcall m1 fd args t m2 res] describes a diverging
   invocation of function [fd] with arguments [args].  *)
 
-with evalinf_funcall: mem -> fundef -> list val -> traceinf -> Prop :=
-  | evalinf_funcall_internal: forall m f vargs t e m1 m2,
+with evalinf_funcall: mem -> fundef -> list val -> traceinf -> ident -> Prop :=
+  | evalinf_funcall_internal: forall m m0 f vargs t e m1 m2 id path,
       list_norepet (var_names f.(fn_params) ++ var_names f.(fn_vars)) ->
-      alloc_variables ge empty_env m (f.(fn_params) ++ f.(fn_vars)) e m1 ->
+      Mem.alloc_frame m id = (m0,path) ->
+      alloc_variables ge empty_env m0 (f.(fn_params) ++ f.(fn_vars)) e m1 ->
       bind_parameters ge e m1 f.(fn_params) vargs m2 ->
       execinf_stmt e m2 f.(fn_body) t ->
-      evalinf_funcall m (Internal f) vargs t.
+      evalinf_funcall m (Internal f) vargs t id.
 
 (** ** Implication from big-step semantics to transition semantics *)
 
@@ -2200,11 +2208,11 @@ Lemma bigstep_to_steps:
    forall f k,
    exists S,
    star step ge (State f s k e m) t S /\ outcome_state_match e m' f k out S)
-/\(forall m fd args t m' res,
-   eval_funcall m fd args t m' res ->
+/\(forall m fd args t m' res id,
+   eval_funcall m fd args t m' res id->
    forall k,
    is_call_cont k ->
-   star step ge (Callstate fd args k m) t (Returnstate res k m')).
+   star step ge (Callstate fd args k m id) t (Returnstate res k m')).
 Proof.
   apply bigstep_induction; intros.
 (* expression, general *)
@@ -2340,14 +2348,14 @@ Proof.
   eexact G.
   reflexivity. traceEq.
 (* call *)
-  exploit (H0 (fun x => C(Ecall x rargs ty))).
+  exploit (H1 (fun x => C(Ecall x rargs ty))).
     eapply leftcontext_compose; eauto. repeat constructor. intros [A [B D]].
-  exploit (H2 rf' Enil ty C); eauto. intros [E F].
+  exploit (H3 rf' Enil ty C); eauto. intros [E F].
   simpl; intuition.
   eapply star_trans. eexact D.
   eapply star_trans. eexact F.
   eapply star_left. left; eapply step_call; eauto. congruence.
-  eapply star_right. eapply H9. red; auto.
+  eapply star_right. eapply H10. red; auto.
   right; constructor.
   reflexivity. reflexivity. reflexivity. traceEq.
 (* nil *)
@@ -2590,22 +2598,22 @@ Proof.
   unfold S2. inv B1; simpl; econstructor; eauto.
 
 (* call internal *)
-  destruct (H3 f k) as [S1 [A1 B1]].
+  destruct (H4 f k) as [S1 [A1 B1]].
   eapply star_left. right; eapply step_internal_function; eauto.
   eapply star_right. eexact A1.
-  inv B1; simpl in H4; try contradiction.
+  inv B1; simpl in H5; try contradiction.
   (* Out_normal *)
   assert (fn_return f = Tvoid /\ vres = Vundef).
     destruct (fn_return f); auto || contradiction.
-  destruct H7 as [P Q]. subst vres. right; eapply step_skip_call; eauto.
+  destruct H9 as [P Q]. subst vres. right; eapply step_skip_call; eauto.
   (* Out_return None *)
   assert (fn_return f = Tvoid /\ vres = Vundef).
     destruct (fn_return f); auto || contradiction.
-  destruct H8 as [P Q]. subst vres.
-  rewrite <- (is_call_cont_call_cont k H6). rewrite <- H7.
-  right; apply step_return_0; auto.
+  destruct H10 as [P Q]. subst vres.
+  rewrite <- (is_call_cont_call_cont k H8). rewrite <- H9.
+  right; eapply step_return_0; eauto.
   (* Out_return Some *)
-  destruct H4. rewrite <- (is_call_cont_call_cont k H6). rewrite <- H7.
+  destruct H5. rewrite <- (is_call_cont_call_cont k H8). rewrite <- H9.
   right; eapply step_return_2; eauto.
   reflexivity. traceEq.
 
@@ -2646,11 +2654,11 @@ Lemma exec_stmt_to_steps:
 Proof (proj1 (proj2 (proj2 (proj2 bigstep_to_steps)))).
 
 Lemma eval_funcall_to_steps:
-  forall m fd args t m' res,
-  eval_funcall m fd args t m' res ->
+  forall m fd args t m' res id,
+  eval_funcall m fd args t m' res id ->
   forall k,
   is_call_cont k ->
-  star step ge (Callstate fd args k m) t (Returnstate res k m').
+  star step ge (Callstate fd args k m id) t (Returnstate res k m').
 Proof (proj2 (proj2 (proj2 (proj2 bigstep_to_steps)))).
 
 Fixpoint esize (a: expr) : nat :=
@@ -2706,9 +2714,9 @@ Proof.
 Qed.
 
 Lemma evalinf_funcall_steps:
-  forall m fd args t k,
-  evalinf_funcall m fd args t ->
-  forever_N step lt ge O (Callstate fd args k m) t.
+  forall m fd args t k id,
+  evalinf_funcall m fd args t id->
+  forever_N step lt ge O (Callstate fd args k m id) t.
 Proof.
   cofix COF.
 
@@ -2875,10 +2883,10 @@ Proof.
   eapply forever_N_star with (a2 := (esizelist a2)). eexact R. simpl; lia.
   eapply COEL with (al := Enil). eauto. auto. auto. auto. traceEq.
 (* call *)
-  destruct (eval_expr_to_steps _ _ _ _ _ _ _ H1 (fun x => C(Ecall x rargs ty)) f k)
+  destruct (eval_expr_to_steps _ _ _ _ _ _ _ H2 (fun x => C(Ecall x rargs ty)) f k)
   as [P [Q R]].
   eapply leftcontext_compose; eauto. repeat constructor.
-  destruct (eval_exprlist_to_steps _ _ _ _ _ _ H2 rf' Enil ty C f k)
+  destruct (eval_exprlist_to_steps _ _ _ _ _ _ H3 rf' Enil ty C f k)
   as [S T]. auto. auto. simpl; auto.
   eapply forever_N_plus. eapply plus_right.
   eapply star_trans. eexact R. eexact T. reflexivity.
@@ -3028,7 +3036,7 @@ Inductive bigstep_program_terminates (p: program): trace -> int -> Prop :=
       Genv.find_symbol ge p.(prog_main) = Some b ->
       Genv.find_funct_ptr ge b = Some f ->
       type_of_fundef f = Tfunction Tnil type_int32s cc_default ->
-      eval_funcall ge m0 f nil t m1 (Vint r) ->
+      eval_funcall ge m0 f nil t m1 (Vint r) p.(prog_main)->
       bigstep_program_terminates p t r.
 
 Inductive bigstep_program_diverges (p: program): traceinf -> Prop :=
@@ -3038,7 +3046,7 @@ Inductive bigstep_program_diverges (p: program): traceinf -> Prop :=
       Genv.find_symbol ge p.(prog_main) = Some b ->
       Genv.find_funct_ptr ge b = Some f ->
       type_of_fundef f = Tfunction Tnil type_int32s cc_default ->
-      evalinf_funcall ge m0 f nil t ->
+      evalinf_funcall ge m0 f nil t p.(prog_main)->
       bigstep_program_diverges p t.
 
 Definition bigstep_semantics (p: program) :=
