x86/Asmgenproof.v
@@ -632,21 +632,22 @@ Opaque loadind.
   exploit lessdef_parent_sp; eauto. intros. subst parent'. clear B.
   exploit lessdef_parent_ra; eauto. intros. subst ra'. clear D.
   exploit Mem.free_parallel_extends; eauto. intros [m2' [E F]].
-  destruct ros as [rf|fid]; simpl in H; monadInv H7.
+  exploit Mem.return_frame_parallel_extends; eauto. intros [m2'' [G I]].
+  destruct ros as [rf|fid]; simpl in H; monadInv H8.
 + (* Indirect call *)
   assert (rs rf = Vptr f' Ptrofs.zero).
     destruct (rs rf); try discriminate.
     revert H; predSpec Ptrofs.eq Ptrofs.eq_spec i Ptrofs.zero; intros; congruence.
   assert (rs0 x0 = Vptr f' Ptrofs.zero).
-    exploit ireg_val; eauto. rewrite H7; intros LD; inv LD; auto.
-  generalize (code_tail_next_int _ _ _ _ NOOV H8). intro CT1.
+    exploit ireg_val; eauto. rewrite H8; intros LD; inv LD; auto.
+  generalize (code_tail_next_int _ _ _ _ NOOV H9). intro CT1.
   left; econstructor; split.
   eapply plus_left. eapply exec_step_internal. eauto.
   eapply functions_transl; eauto. eapply find_instr_tail; eauto.
   simpl. replace (chunk_of_type Tptr) with Mptr in * by (unfold Tptr, Mptr; destruct Archi.ptr64; auto).
-  rewrite C. rewrite A. rewrite <- (sp_val _ _ _ AG). rewrite E. eauto.
+  rewrite C. rewrite A. rewrite <- (sp_val _ _ _ AG). rewrite E. eauto. rewrite G. eauto.
   apply star_one. eapply exec_step_internal.
-  transitivity (Val.offset_ptr rs0#PC Ptrofs.one). auto. rewrite <- H4. simpl. eauto.
+  transitivity (Val.offset_ptr rs0#PC Ptrofs.one). auto. rewrite <- H5. simpl. eauto.
   eapply functions_transl; eauto. eapply find_instr_tail; eauto.
   simpl. eauto. traceEq.
   econstructor; eauto.
@@ -655,14 +656,14 @@ Opaque loadind.
   Simplifs. rewrite Pregmap.gso; auto.
   generalize (preg_of_not_SP rf). rewrite (ireg_of_eq _ _ EQ1). congruence.
 + (* Direct call *)
-  generalize (code_tail_next_int _ _ _ _ NOOV H8). intro CT1.
+  generalize (code_tail_next_int _ _ _ _ NOOV H9). intro CT1.
   left; econstructor; split.
   eapply plus_left. eapply exec_step_internal. eauto.
   eapply functions_transl; eauto. eapply find_instr_tail; eauto.
   simpl. replace (chunk_of_type Tptr) with Mptr in * by (unfold Tptr, Mptr; destruct Archi.ptr64; auto).
-  rewrite C. rewrite A. rewrite <- (sp_val _ _ _ AG). rewrite E. eauto.
+  rewrite C. rewrite A. rewrite <- (sp_val _ _ _ AG). rewrite E. eauto. rewrite G. eauto.
   apply star_one. eapply exec_step_internal.
-  transitivity (Val.offset_ptr rs0#PC Ptrofs.one). auto. rewrite <- H4. simpl. eauto.
+  transitivity (Val.offset_ptr rs0#PC Ptrofs.one). auto. rewrite <- H5. simpl. eauto.
   eapply functions_transl; eauto. eapply find_instr_tail; eauto.
   simpl. eauto. traceEq.
   econstructor; eauto.
@@ -816,14 +817,15 @@ Transparent destroyed_by_jumptable.
   exploit Mem.loadv_extends. eauto. eexact H1. auto. simpl. intros [ra' [C D]].
   exploit lessdef_parent_ra; eauto. intros. subst ra'. clear D.
   exploit Mem.free_parallel_extends; eauto. intros [m2' [E F]].
-  monadInv H6.
+  exploit Mem.return_frame_parallel_extends; eauto. intros [m2'' [G I]].
+  monadInv H7.
   exploit code_tail_next_int; eauto. intro CT1.
   left; econstructor; split.
   eapply plus_left. eapply exec_step_internal. eauto.
   eapply functions_transl; eauto. eapply find_instr_tail; eauto.
-  simpl. rewrite C. rewrite A. rewrite <- (sp_val _ _ _ AG). rewrite E. eauto.
+  simpl. rewrite C. rewrite A. rewrite <- (sp_val _ _ _ AG). rewrite E. eauto. rewrite G. eauto.
   apply star_one. eapply exec_step_internal.
-  transitivity (Val.offset_ptr rs0#PC Ptrofs.one). auto. rewrite <- H3. simpl. eauto.
+  transitivity (Val.offset_ptr rs0#PC Ptrofs.one). auto. rewrite <- H4. simpl. eauto.
   eapply functions_transl; eauto. eapply find_instr_tail; eauto.
   simpl. eauto. traceEq.
   constructor; auto.
@@ -836,16 +838,18 @@ Transparent destroyed_by_jumptable.
   destruct (zlt Ptrofs.max_unsigned (list_length_z (fn_code x0))); inv EQ1.
   monadInv EQ0. rewrite transl_code'_transl_code in EQ1.
   unfold store_stack in *.
+  exploit Mem.alloc_frame_extends; eauto. intros [m0' [A' B']].
   exploit Mem.alloc_extends. eauto. eauto. apply Z.le_refl. apply Z.le_refl.
   intros [m1' [C D]].
-  exploit Mem.storev_extends. eexact D. eexact H1. eauto. eauto.
+  exploit Mem.storev_extends. eexact D. eexact H2. eauto. eauto.
   intros [m2' [F G]].
-  exploit Mem.storev_extends. eexact G. eexact H2. eauto. eauto.
+  exploit Mem.storev_extends. eexact G. eexact H3. eauto. eauto.
   intros [m3' [P Q]].
   left; econstructor; split.
   apply plus_one. econstructor; eauto.
   simpl. rewrite Ptrofs.unsigned_zero. simpl. eauto.
-  simpl. rewrite C. simpl in F, P.
+  Opaque Mem.alloc_frame.
+  simpl. rewrite A'. rewrite C. simpl in F, P.
   replace (chunk_of_type Tptr) with Mptr in F, P by (unfold Tptr, Mptr; destruct Archi.ptr64; auto).
   rewrite (sp_val _ _ _ AG) in F. rewrite F.
   rewrite ATLR. rewrite P. eauto.
@@ -873,7 +877,7 @@ Transparent destroyed_at_function_entry.
   eapply external_call_symbols_preserved; eauto. apply senv_preserved.
   econstructor; eauto.
   unfold loc_external_result. apply agree_set_other; auto. apply agree_set_pair; auto.
-  apply agree_undef_caller_save_regs; auto. 
+  apply agree_undef_caller_save_regs; auto.
 
 - (* return *)
   inv STACKS. simpl in *.
